%\chapterimage{head2.png} % Chapter heading image
%\appendix{Integrals}


\ifpdf
\graphicspath{{Appendix1/figs/}}
\else
\graphicspath{{Appendix1/figs/}}
\fi
\chapter{Standard Integrals} 
\label{appendix1.Integrals}

\section{List of Standard Integrals}
\begin{align}
\label{appendix1.eqn1}
\int_{-\infty}^{\infty} e^{-x^2} \dd{x} &= \sqrt{\pi} \\
\label{appendix1.eqn2}
\int_{-\infty}^{\infty} e^{-ax^2} \dd{x} &=  \sqrt{\frac{\pi}{a}} \\
\label{appendix1.eqn3}
\int_{-\infty}^{\infty} x^2 e^{-ax^2}  \dd{x} &= \frac{1}{2 a} \sqrt{\frac{\pi}{a}} \\
\label{appendix1.eqn4}
\int_{-\infty}^{\infty} x^4 e^{-ax^2}  \dd{x} &= \frac{3}{4 a^2} \sqrt{\frac{\pi}{a}} \\
\label{appendix1.eqn5}
\int_{-\infty}^{\infty} x^{2 n} e^{-ax^2}  \dd{x} &=  \frac{1\cdot 2 \cdot 3 \cdots \qty(2n - 1)}{2^n a^n}\sqrt{\frac{\pi}{a}} \quad n=0,1,\ldots
\end{align}




\begin{equation}
\int_{-\infty}^{\infty} e^{-\alpha x^2 + \beta x} \dd{x} = \left(\frac{\pi}{2}\right)^{1/2} \exp\left[\frac{\beta^2}{4\alpha}\right]
\label{appendix1.eqn6}
\end{equation}


\section{Proofs}
\begin{equation}
	\int_{-\infty}^{\infty} e^{-x^2} \dd{x} = \sqrt{\pi}
\end{equation}
proof:\\
let,
\begin{equation}
	I = \int_{-\infty}^{\infty} e^{-x^2} \dd{x} 
\end{equation}
then
\begin{eqnarray}
	I^2 = \int_{-\infty}^{\infty}\int_{-\infty}^{\infty} e^{-(x^2+y^2)} \dd{x} dd{y}
\end{eqnarray}
using $r^2 = x^2 + y^2$ since
\begin{eqnarray}
	x &= r \cos \theta \\
	y &= r \sin \theta
\end{eqnarray}
we get 
\begin{eqnarray}
	I^2 
	&= \int_{0}^{2 \pi}\int_{0}^{\infty} e^{-r^2} r \dd{r} dd{\theta} \\
	&= 2 \pi \int_{0}^{\infty} e^{-r^2} r \dd{r}
\end{eqnarray}
let $u = r^2$ therefore $rdr = du/2$
\begin{align}
I^2 
&=  \pi \int_{0}^{\infty} e^{-u} \dd{u} \\
&=  \pi \left[\frac{e^{-u}}{-1} \right]_{0}^{\infty} \\
&= \pi \left[0 - (-1)\right] \\
&= \pi
\end{align}
therefore $I=\sqrt{\pi}$\\
\textbf{another}\\
\begin{eqnarray}
I = \int_{-\infty}^{\infty} \dd{x} \  e^{-\left(b^2 x^2 + a x\right)}
\end{eqnarray}
Notice that $\left(b^2 x^2 + a x\right) = (b x + \frac{a}{2 b})^2 - \frac{a^2}{4b^2}$
\begin{eqnarray}
I = e^{a^2/4b^2}\int_{-\infty}^{\infty} \dd{x}\ e^{-(b x + \frac{a}{2 b})^2}
\end{eqnarray}
let $z = b x + \frac{a}{2 b}$ thus $\dd{z} = b \dd{x}$
\begin{eqnarray}
I 
&= e^{a^2/4b^2} \frac{1}{b} \int_{-\infty}^{\infty} \dd{z}\  e^{-z^2} \\
&= e^{a^2/4b^2} \frac{\sqrt{\pi}}{b}
\end{eqnarray}

\section{Gamma Beta functions}
\begin{equation}
	\Gamma\qty(n+1) = \int_0^\infty x^n e^{-x} \dd{x} = n!
\end{equation}
\begin{align}
\int_{0}^{\infty} x^n e^{-\beta x} \dd{x} = \frac{\Gamma\qty(n+1)}{\beta^{n+1}} = \frac{n!}{\beta^{n+1}}
\end{align}


\section{From Chapter 21}
\begin{align}
	\int e^{-x} \dd{x} &= - e^{-x} \\
	\int x e^{-x} \dd{x} &= - \qty(1 + x) e^{-x} \\
	\int x^2 e^{-x} \dd{x} &= -\qty(2 + 2 x + x^2)  e^{-x}
\end{align}